Here are the solutions to the 30 algebra questions.

### **Answers for Algebra 1**

1.  **Answer**: 21
    * [cite_start]$a(c-b) = 3(5 - (-2)) = 3(5+2) = 3(7) = 21$ [cite: 1315]

2.  **Answer**: 18
    * [cite_start]$x^2 - 3x = (-3)^2 - 3(-3) = 9 - (-9) = 9 + 9 = 18$ [cite: 1398]

3.  **Answer**: $6x^2 - 2x$
    * [cite_start]$7x + 3x(2x-3) = 7x + 6x^2 - 9x = 6x^2 - 2x$ [cite: 1571, 1574]

4.  **Answer**: $x^2 + 8x + 15$
    * [cite_start]$(x+5)(x+3) = x(x+3) + 5(x+3) = x^2 + 3x + 5x + 15 = x^2 + 8x + 15$ [cite: 1620]

5.  **Answer**: $x = 18$
    * [cite_start]$5x - 3(x-1) = 39 \implies 5x - 3x + 3 = 39 \implies 2x = 36 \implies x = 18$ [cite: 1796]

6.  **Answer**: $x = 2$
    * [cite_start]$(x+3)^2 = (x+2)^2 + 9 \implies x^2+6x+9 = (x^2+4x+4) + 9 \implies 6x+9 = 4x+13 \implies 2x=4 \implies x=2$ [cite: 1817]

7.  **Answer**: $x = \frac{13}{5}$ or $2.6$
    * [cite_start]$\frac{x+3}{4} = \frac{2x-1}{3} \implies 3(x+3) = 4(2x-1) \implies 3x+9 = 8x-4 \implies 13 = 5x \implies x = \frac{13}{5}$ [cite: 1857]

8.  **Answer**: The numbers are 25, 26, and 27.
    * Let the numbers be $x, x+1, x+2$.
    * [cite_start]$x + (x+1) + (x+2) = 78 \implies 3x+3=78 \implies 3x=75 \implies x=25$ [cite: 1930]

9.  **Answer**: $x=2, y=1$
    * From $2x+y=5$, we get $y=5-2x$.
    * Substitute into the second equation: $3x - 2(5-2x) = 4 \implies 3x - 10 + 4x = 4 \implies 7x=14 \implies x=2$.
    * [cite_start]Substitute $x=2$ back into $y=5-2x \implies y=5-4=1$. [cite: 2128]

10. **Answer**: $x=4, y=2$
    * Multiply the first equation by 2: $2(x+2y) = 2(8) \implies 2x+4y=16$.
    * Subtract the second equation from this: $(2x+4y)-(2x+3y)=16-14 \implies y=2$.
    * [cite_start]Substitute $y=2$ back into $x+2y=8 \implies x+4=8 \implies x=4$. [cite: 2132, 2133]

---
### **Answers for Algebra 2**

1.  **Answer**: $(a+b)(h+k)$
    * [cite_start]$ah+ak+bh+bk = a(h+k) + b(h+k) = (a+b)(h+k)$ [cite: 84, 90]

2.  **Answer**: $(x+5)(x-3)$
    * You need two numbers that multiply to -15 and add to +2. [cite_start]These are +5 and -3. [cite: 131, 136]

3.  **Answer**: $(5m-9n)(5m+9n)$
    * [cite_start]This is a difference of two squares: $(5m)^2 - (9n)^2$. [cite: 238, 248, 249]

4.  **Answer**: $x = \frac{1}{2}$ or $x = -\frac{2}{3}$
    * [cite_start]$6x^2+x-2=0 \implies (2x-1)(3x+2)=0$. [cite: 368, 369]

5.  **Answer**: $x = \frac{3 + \sqrt{41}}{4}$ or $x = \frac{3 - \sqrt{41}}{4}$
    * Using $x = \frac{-b \pm \sqrt{b^2 - 4ac}}{2a}$ with $a=2, b=-3, c=-4$.
    * [cite_start]$x = \frac{3 \pm \sqrt{(-3)^2 - 4(2)(-4)}}{2(2)} = \frac{3 \pm \sqrt{9+32}}{4} = \frac{3 \pm \sqrt{41}}{4}$ [cite: 464, 472]

6.  **Answer**: $x = 5 + \sqrt{42}$ or $x = 5 - \sqrt{42}$
    * [cite_start]$x^2-10x-17=0 \implies (x-5)^2 - 5^2 - 17 = 0 \implies (x-5)^2 - 42 = 0 \implies (x-5)^2=42 \implies x = 5 \pm \sqrt{42}$ [cite: 579, 584]

7.  **Answer**: The numbers are 8 and 11.
    * Let the numbers be *x* and *x*+3. Their product is $x(x+3)=88$.
    * $x^2+3x-88=0 \implies (x+11)(x-8)=0$. [cite_start]Since the numbers are positive, $x=8$. [cite: 682]

8.  **Answer**: The length is 12 cm.
    * Let the width be *w*. The length is *w*+7. Area is $w(w+7)=60$.
    * $w^2+7w-60=0 \implies (w+12)(w-5)=0$. Since width must be positive, $w=5$.
    * [cite_start]The length is $5+7=12$ cm. [cite: 689, 690]

9.  **Answer**: $(x,y) = (-3, -2)$ and $(1, 2)$
    * Substitute $y=x+1$ into the second equation: $x+1 = x^2+3x-2$.
    * $0 = x^2+2x-3 \implies 0=(x+3)(x-1)$. So $x=-3$ or $x=1$.
    * If $x=-3, y=-3+1=-2$. [cite_start]If $x=1, y=1+1=2$. [cite: 730, 740, 742, 744]

10. **Answer**: $(x,y) = (-0.31, -3.63)$ and $(-3.19, -9.37)$
    * From $2x-y=3$, we get $y=2x-3$. Substitute into the second equation: $2x-3=2x^2+9x-1$.
    * $0=2x^2+7x+2$. Using the quadratic formula, $x = \frac{-7 \pm \sqrt{7^2-4(2)(2)}}{4} = \frac{-7 \pm \sqrt{33}}{4}$.
    * $x \approx -0.31$ or $x \approx -3.19$.
    * If $x \approx -0.31, y \approx 2(-0.31)-3 = -3.62$. [cite_start]If $x \approx -3.19, y \approx 2(-3.19)-3 = -9.38$. [cite: 746, 762, 784]

---
### **Answers for Algebra 3**

1.  **Answer**: $\frac{x-2}{x-1}$
    * [cite_start]$\frac{x^2+x-6}{x^2+2x-3} = \frac{(x+3)(x-2)}{(x+3)(x-1)} = \frac{x-2}{x-1}$ [cite: 2251]

2.  **Answer**: $\frac{9x-3}{20}$
    * [cite_start]$\frac{5(x+1)}{20} + \frac{4(x-2)}{20} = \frac{5x+5+4x-8}{20} = \frac{9x-3}{20}$ [cite: 2333]

3.  **Answer**: $a = \frac{T}{M} - B$
    * [cite_start]$M(a+B)=T \implies a+B = \frac{T}{M} \implies a = \frac{T}{M} - B$ [cite: 2495]

4.  **Answer**: $y=\frac{5x}{3}$
    * [cite_start]$\sqrt{\frac{y+x}{y-x}} = 2 \implies \frac{y+x}{y-x}=4 \implies y+x = 4(y-x) \implies y+x=4y-4x \implies 5x=3y \implies y=\frac{5x}{3}$ [cite: 2691]

5.  **Answer**: $1800
    * $V \propto M^2 \implies V=kM^2$. Given $200=k(10^2) \implies k=2$.
    * The formula is $V=2M^2$. [cite_start]When $M=30$, $V=2(30^2)=2(900)=1800$. [cite: 2771, 2785]

6.  **Answer**: 6 cm
    * $F \propto \frac{1}{d^2} \implies F = \frac{k}{d^2}$. Given $18 = \frac{k}{2^2} \implies k=72$.
    * The formula is $F = \frac{72}{d^2}$. [cite_start]When $F=2$, $2 = \frac{72}{d^2} \implies d^2=36 \implies d=6$. [cite: 2973, 2975]

7.  **Answer**: $4x^3$
    * [cite_start]$(2x^{-1})^2 \div x^{-5} = (4x^{-2}) \div x^{-5} = 4x^{-2 - (-5)} = 4x^3$ [cite: 2995]

8.  **Answer**: $x=-2$
    * [cite_start]$4^{x-1} = 8^x \implies (2^2)^{x-1} = (2^3)^x \implies 2^{2x-2} = 2^{3x} \implies 2x-2=3x \implies x=-2$ [cite: 3126, 3135]

9.  **Answer**: $x \ge \frac{4}{3}$
    * $5-3x \le 1 \implies -3x \le -4$. [cite_start]Divide by -3 and reverse the inequality sign. [cite: 3197, 3201]

10. **Answer**: The integers are 2, 3, 4, 5, 6.
    * Solve as two parts: $x < 3x+2 \implies -2 < 2x \implies -1 < x$.
    * And $3x+2 < 2x+6 \implies x < 4$.
    * Combining gives $-1 < x < 4$. [cite_start]The integers are 0, 1, 2, 3. [cite: 3274]